Program-proofs/Exercises/2D-counting/prob13/prob13.dfy
@@ -4,7 +4,7 @@
    This is exercise 9.15 from the PC reader
 */            
 
-ghost predicate pos(f: (nat) -> nat)
+ghost predicate posFunc(f: (nat) -> nat)
 {
     // Expresses the property that f is a positive function, 
     // i.e. f(k) > 0 for all k in the domain of f.
@@ -12,10 +12,10 @@ ghost predicate pos(f: (nat) -> nat)
 }
 
 method problem13(f: (nat) -> nat, a: nat, n: nat)
-returns (r: nat)
+returns (z: nat)
 requires 0 < a && 0 < n
-requires pos(f)
-ensures r == ???
+requires posFunc(f)
+ensures z == ???
 {
   /*
     Given is a function f: ℕ → ℕ₊. Derive a command sequence T that 
@@ -26,12 +26,12 @@ ensures r == ???
       
         {P : Z = #{ (i,j) | i,j: 0 ≤ i ≤ j < n ∧ a = ∑( f(k) | k: i ≤ k < j ) }}
       T
-        {Q : Z = r}
+        {Q : Z = z}
       
     In other words, the program should compute the total number of contiguous 
     subsequences taken from the sequence f(0), f(1), ..., f(n-2) that sum to a.
     Note that Z (uppercase) is a specification constant, not a program 
-    variable, whereas r (lowercase) is a program variable.
+    variable, whereas z (lowercase) is a program variable.
     The time complexity of T should be in O(n).
   */
 }
