Program-proofs/Exercises/2D-counting/prob13/sol13PCStyleAnnotated.dfy
@@ -1,51 +1,44 @@
-/* file: sol13Annotated.dfy
-   author: David De Potter
-   description: extra practice in Dafny, 2D-counting, 
-   solution to prob13, with annotations
-   This is exercise 9.15 from the PC reader
-   NOTE: The loop is machine-verified against the recursive definition of F. 
-    The connection between F(f,0,0,a,n) and the set-based specification from the 
-    problem statement is manually derived and justified in the comments, but 
-    not machine-verified. This avoids the additional technical machinery that 
-    would be needed in Dafny to introduce the corresponding finite sets, 
-    reason about their cardinalities, and prove the equivalence of the 
-    set-based specification and the recursive definition of F. It also keeps 
-    the solution in line with the PC lecture notes.
+/*  file: sol13PCStyleAnnotated.dfy
+    author: David De Potter
+    description: extra practice in Dafny, 2D-counting, 
+    solution to prob13, with annotations
+    This is exercise 9.15 from the PC reader
+    NOTE: This solution follows the PC-style proof method described
+    in the general note on proof styles (see the README in the 
+    Exercises folder)
 */
 
-ghost predicate Pos(f: (nat) -> nat)
+include "../../commonSupport.dfy"
+import opened CommonFunctions
+
+ghost predicate posFunc(f: (nat) -> nat)
 {
     // Expresses the property that f is a positive function, 
     // i.e. f(k) > 0 for all k in the domain of f.
   (forall k:: f(k) > 0)
 }
 
-function Ord(b:bool): nat
-{
-  if b then 1 else 0
-}
-
 ghost function F(f: (nat) -> nat, x: nat, y: nat, a: nat, n: nat): nat
-requires Pos(f)
+requires posFunc(f)
 requires 0 < a 
 decreases 2 * n - y - x
 {
     // We want to find a recursive definition of F that we can use to derive T.
     // We define F as follows:
     //   F(f,x,y,a,n) 
-    //      = #{ (i,j) | i,j: x ≤ i ≤ j < n ∧ y ≤ j ∧ a = ∑( f(k) | k: i ≤ k < j ) }
-    //      = #{ (i,j) | i,j: x ≤ i ≤ j < n ∧ y ≤ j ∧ a = S(f,i,j) }
+    //   = #{ (i,j) | i,j: x ≤ i ≤ j < n ∧ y ≤ j ∧ a = ∑( f(k) | k: i ≤ k < j )}
+    //   = #{ (i,j) | i,j: x ≤ i ≤ j < n ∧ y ≤ j ∧ a = S(f,i,j) }
     //
-    // In other words, F(f,x,y,a,n) counts the number of remaining half-open intervals 
-    // [i,j) for which the sum of the values of f on the interval equals a. 
-    // In the initial call F(f,0,0,a,n), this is the full search region from the 
-    // problem statement.
+    // In other words, F(f,x,y,a,n) counts the number of remaining half-open  
+    // intervals [i,j) for which the sum of the values of f on the interval 
+    // equals a. In the initial call F(f,0,0,a,n), this is the full search 
+    // region from the problem statement.
     //
     // Base case: if y ≥ n or x ≥ n, then the remaining search area is empty, 
     //   so F(f,x,y,a,n) = # ∅ = 0.
     // Recursive case: here we want to shrink the remaining search area by 
-    //   - either incrementing x (which removes the leftmost element) 
-    //   - or incrementing y (which adds a new rightmost element)
+    //   - either incrementing x (which shrinks the search area from the left)
+    //   - or incrementing y (which shrinks the search area from the bottom)
     //
     // What happens if we increment x?
     //   F(f,x,y,a,n)
@@ -61,8 +54,8 @@ decreases 2 * n - y - x
     //        ( S(f,x,j) is increasing in j, so the value of S(f,x,y) is minimal;
     //          if we assume S(f,x,y) ≥ a, then only the interval [x,y) can sum 
     //          to a, since S(f,x,j) > S(f,x,y) ≥ a for all j > y. Hence, we can 
-    //          increment the count by 1 iff S(f,x,y) = a, or ignore all intervals 
-    //          starting at x if S(f,x,y) > a )
+    //          increment the count by 1 iff S(f,x,y) = a, or ignore all  
+    //          intervals starting at x if S(f,x,y) > a )
     //   = F(f,x+1,y,a,n) + (S(f,x,y) = a ? 1 : 0)
     //
     // What happens if we increment y?
@@ -75,14 +68,14 @@ decreases 2 * n - y - x
     //   = F(f,x,y+1,a,n) + #{ (i,y) | i: x ≤ i ≤ y < n ∧ a = S(f,i,y) }
     //        ( S(f,i,y) is decreasing in i, so the value of S(f,x,y) is maximal;
     //          if we assume S(f,x,y) < a, then S(f,i,y) ≤ S(f,x,y) < a for all
-    //          i with x ≤ i ≤ y, and hence we can ignore all intervals ending at y
-    //          as they cannot sum to a )
+    //          i with x ≤ i ≤ y, and hence we can ignore all intervals ending 
+    //          at y as they cannot sum to a )
     //   = F(f,x,y+1,a,n) + # ∅
     //        ( size of the empty set is 0 )
     //   = F(f,x,y+1,a,n)
   if y >= n || x >= n then 0
   else if S(f,x,y) >= a 
-       then F(f,x+1,y,a,n) + Ord(S(f,x,y) == a)
+       then F(f,x+1,y,a,n) + ord(S(f,x,y) == a)
        else F(f,x,y+1,a,n)
 }
 
@@ -91,14 +84,14 @@ decreases y - x
 {
     // We define S(f,x,y) = ∑( f(k) | k: x ≤ k < y )
     // Base case: if x ≥ y, then the sum is empty, so S(f,x,y) = 0.
-    // Recursive case: if x < y, then we can split the non-empty domain 
-    //   and derive the recursive case as follows:
+    // Recursive case: if x < y, then we can split the non-empty  
+    // domain and derive the recursive case as follows:
     //  S(f,x,y)
     //    = ∑( f(k) | k: x ≤ k < y )
     //        ( split domain into x + 1 ≤ k < y and k = x )
-    //    = ∑( f(k) | k: x + 1 ≤ k < y ) + f(x)
+    //    = f(x) + ∑( f(k) | k: x + 1 ≤ k < y )
     //        ( apply definition of S to the first term )
-    //    = S(f,x+1,y) + f(x)
+    //    = f(x) + S(f,x+1,y)
   if x >= y then 0 else f(x) + S(f,x+1,y)
 }
 
@@ -107,7 +100,7 @@ requires x <= y
 ensures S(f,x,y+1) == S(f,x,y) + f(y)
 decreases y - x
 {
-    // We prove the lemma by induction on the length of the 
+    // We prove the lemma by induction on the length l of the 
     // half-open interval [x,y), l = y - x.
     // The statement to prove is: S(f,x,y+1) = S(f,x,y) + f(y)
     // That is: extending the upper bound of the half-open interval
@@ -146,12 +139,12 @@ decreases y - x
 method problem13(f: (nat) -> nat, a: nat, n: nat)
 returns (z: nat)
 requires 0 < a && 0 < n
-requires Pos(f)
+requires posFunc(f)
 ensures z == F(f,0,0,a,n)
 {
     // Initialization to establish J before the loop
     // P: F(f,0,0,a,n) = Z
-    //   ( arithmetic )
+    //   ( arithmetic; base case of S is applicable since x = y = 0 )
     // 0 + F(f,0,0,a,n) = Z ∧ 0 = S(f,0,0)
   var x, y, s := 0, 0, 0;
   z := 0;
@@ -164,8 +157,9 @@ ensures z == F(f,0,0,a,n)
   {
       // J ∧ B ∧ vf = V
       // z + F(f,x,y,a,n) = Z ∧ s = S(f,x,y) ∧ x < n ∧ y < n ∧ 2 * n - x - y = V
-      //   ( we want to apply the definition of F. Since we are not in the base case,
-      //     we need to distinguish the recursive cases S(f,x,y) ≥ a and S(f,x,y) < a )
+      //   ( we want to apply the definition of F. Since we are not in the base 
+      //     case, we need to distinguish the recursive cases S(f,x,y) ≥ a 
+      //     and S(f,x,y) < a )
 
     if s >= a
     {
@@ -174,10 +168,10 @@ ensures z == F(f,0,0,a,n)
         //   ( apply definition of F )
         // z + F(f,x+1,y,a,n) + (S(f,x,y) = a ? 1 : 0) = Z ∧ s = S(f,x,y)
         //   ∧ 2 * n - x - y = V
-      z := z + Ord(s == a);
+      z := z + ord(s == a);
         // z + F(f,x+1,y,a,n) = Z ∧ s = S(f,x,y) ∧ 2 * n - x - y = V
-        //   ( apply definition of S to update s; the recursive case of S is applicable
-        //     since x < y, which follows from S(f,x,y) ≥ a > 0 )
+        //   ( apply definition of S to update s; the recursive case of S is 
+        //     applicable since x < y, which follows from S(f,x,y) ≥ a > 0 )
         // z + F(f,x+1,y,a,n) = Z ∧ s - f(x) = S(f,x+1,y) ∧ 2 * n - x - y = V
       s := s - f(x);
         // z + F(f,x+1,y,a,n) = Z ∧ s = S(f,x+1,y) ∧ 2 * n - x - y = V
